testdata/modules/dup_import_binding/main.cue
@@ -1,0 +1,5 @@
+package main
+
+import "example.com/parts"
+
+out: parts.#Metadata & {#name: "n"}
