testdata/modules/dup_import_binding/parts/other.cue
@@ -1,0 +1,5 @@
+package parts
+
+import "example.com/attr"
+
+#Other: attr.#Metadata
